examples/seplogic/SepLogic.Heap.fsti
@@ -8,9 +8,8 @@ let set  = Set.set
 (* heaps, memories, and operations on them *)
 
 val heap : Type u#1
-val raw_memory : Type u#1
-val defined : raw_memory -> Type0
-let memory = m:raw_memory{defined m}
+val memory : Type u#1
+val defined : memory -> Type0
 
 val emp : memory
 
@@ -24,20 +23,20 @@ val addr_of : #a:Type0 -> ref a -> GTot nat
 val heap_memory : heap -> GTot memory
 
 val disjoint_heaps : heap -> heap -> Type0
-val disjoint_memories : raw_memory -> raw_memory -> Type0
+val disjoint_memories : memory -> memory -> Type0
 
 val join : h0:heap -> h1:heap{disjoint_heaps h0 h1} -> Tot heap
 
 val ( |> ) : #a:Type0 -> r:ref a -> x:a -> GTot memory
-val ( <*> ) : m0:raw_memory -> m1:raw_memory -> GTot raw_memory
+val ( <*> ) : m0:memory -> m1:memory -> GTot memory
 
-val split_heap : (m0:raw_memory) 
-              -> (m1:raw_memory)
+val split_heap : (m0:memory) 
+              -> (m1:memory)
               -> (h:heap{defined (m0 <*> m1) /\ heap_memory h == (m0 <*> m1)}) 
               -> heap * heap
 
 val hcontains : #a:Type0 -> heap -> ref a -> Type0
-val mcontains : #a:Type0 -> raw_memory -> ref a -> Type0
+val mcontains : #a:Type0 -> memory -> ref a -> Type0
 
 val sel : #a:Type0 -> h:heap -> r:ref a{h `hcontains` r} -> Tot a
 val upd : #a:Type0 -> h:heap -> r:ref a{h `hcontains` r} -> x:a -> Tot heap
@@ -45,19 +44,19 @@ val upd : #a:Type0 -> h:heap -> r:ref a{h `hcontains` r} -> x:a -> Tot heap
 val fresh : #a:Type0 -> ref a -> heap -> Type0
 val alloc : #a:Type0 -> h:heap -> a -> Tot (ref a * heap) 
 
-val addrs_in : raw_memory -> Set.set nat
+val addrs_in : memory -> Set.set nat
 
 (* disjoint_heaps and disjoint_memories *)
 
 val lemma_disjoint_heaps_comm (h0 h1:heap)
   : Lemma (disjoint_heaps h0 h1 <==> disjoint_heaps h1 h0)
 
-val lemma_disjoint_memories_emp (m:raw_memory)
+val lemma_disjoint_memories_emp (m:memory)
   : Lemma (requires (defined m))
           (ensures  (disjoint_memories m emp))
           [SMTPat (disjoint_memories m emp)]
 
-val lemma_disjoint_memories_comm (m0 m1:raw_memory)
+val lemma_disjoint_memories_comm (m0 m1:memory)
   : Lemma (requires (defined m0 /\ defined m1))
           (ensures  (disjoint_memories m0 m1 <==> disjoint_memories m1 m0))
 
@@ -65,7 +64,7 @@ val lemma_disjoint_heaps_memories (h0 h1:heap)
   : Lemma (disjoint_heaps h0 h1 <==> disjoint_memories (heap_memory h0) (heap_memory h1))
           [SMTPat (disjoint_memories (heap_memory h0) (heap_memory h1))]
 
-val lemma_sep_disjoint_memories (m0 m1:raw_memory) 
+val lemma_sep_disjoint_memories (m0 m1:memory) 
   : Lemma (disjoint_memories m0 m1 <==> defined (m0 <*> m1))
           [SMTPat (disjoint_memories m0 m1);
            SMTPat (defined (m0 <*> m1))]
@@ -78,14 +77,14 @@ val lemma_join_comm (h0 h1:heap)
 
 (* <*> *)
 
-val lemma_sep_unit (m:raw_memory)
+val lemma_sep_unit (m:memory)
   : Lemma ((m <*> emp) == m)
           [SMTPat (m <*> emp)]
 
-val lemma_sep_comm (m0 m1:raw_memory)
+val lemma_sep_comm (m0 m1:memory)
   : Lemma ((m0 <*> m1) == (m1 <*> m0))
           
-val lemma_sep_assoc (m0 m1 m2:raw_memory)
+val lemma_sep_assoc (m0 m1 m2:memory)
   : Lemma ((m0 <*> (m1 <*> m2)) == ((m0 <*> m1) <*> m2))
          [SMTPatOr [[SMTPat ((m0 <*> (m1 <*> m2)))];
 	            [SMTPat ((m0 <*> m1) <*> m2)]]]
@@ -103,25 +102,25 @@ val lemma_points_to_defined (#a:Type0) (r:ref a) (x:a)
   : Lemma (defined (r |> x))
           [SMTPat (defined (r |> x))]
 
-val lemma_sep_defined (m0 m1:raw_memory)
-  : Lemma (requires (defined (m0 <*> m1)))
-          (ensures  (defined m0 /\ defined m1))
+val lemma_sep_defined (m0 m1:memory)
+  : Lemma (defined (m0 <*> m1) <==> (defined m0 /\ defined m1 /\ Set.disjoint (addrs_in m0) (addrs_in m1)))
+ 	  [SMTPat (defined (m0 <*> m1))]
 
 (* split_heap *)
 
-val lemma_split_heap_disjoint (m0 m1:raw_memory) (h:heap)
+val lemma_split_heap_disjoint (m0 m1:memory) (h:heap)
   : Lemma (requires (defined (m0 <*> m1) /\ heap_memory h == (m0 <*> m1)))
           (ensures  (let (h0,h1) = split_heap m0 m1 h in
                      disjoint_heaps h0 h1))
           [SMTPat (split_heap m0 m1 h)]
 
-val lemma_split_heap_join (m0 m1:raw_memory) (h:heap)
+val lemma_split_heap_join (m0 m1:memory) (h:heap)
   : Lemma (requires (defined (m0 <*> m1) /\ heap_memory h == (m0 <*> m1)))
           (ensures  (let (h0,h1) = split_heap m0 m1 h in
                      h == join h0 h1))
           [SMTPat (split_heap m0 m1 h)]
 
-val lemma_split_heap_memories (m0 m1:raw_memory) (h:heap)
+val lemma_split_heap_memories (m0 m1:memory) (h:heap)
   : Lemma (requires (defined (m0 <*> m1) /\ heap_memory h == (m0 <*> m1)))
           (ensures  (let (h0,h1) = split_heap m0 m1 h in
                      heap_memory h0 == m0 /\ heap_memory h1 == m1))
@@ -187,7 +186,7 @@ val lemma_addrs_in_points_to (#a:Type) (r:ref a) (x:a)
   : Lemma (Set.equal (addrs_in (r |> x)) (Set.singleton (addr_of r)))
           [SMTPat (addrs_in (r |> x))]
 
-val lemma_addrs_in_join (m0 m1:raw_memory)
+val lemma_addrs_in_join (m0 m1:memory)
   : Lemma (requires (defined (m0 <*> m1)))
           (ensures  (Set.equal (addrs_in (m0 <*> m1)) (Set.union (addrs_in m0) (addrs_in m1))))
           [SMTPat (addrs_in (m0 <*> m1))]
